2. Show that $\lnot(p\lor q)\equiv\lnot p\land\lnot q$  
$\lnot p\land\lnot q$  
$\equiv \lnot[\lnot(\lnot p)\lor\lnot(\lnot q)]$ since $p\land q\equiv\lnot(\lnot p\lor\lnot q)$  
$\equiv\lnot(p\lor q)$

3. truth table  
4. Show that these hold:
    1. (shown)
    2. $(p\land q)\lor r\equiv(p\lor r)\land(q\lor r)$  
        $(p\lor r)\land(q\lor r)$  
        $\equiv (p\land q)\lor(p\land r)\lor(r\land q)\lor(r\land r)$  
        $\equiv (p\land q)\lor (r\lor(p\land r))\lor(r\land q)$  
        $\equiv (p\land q)\lor (r\lor(r\land q))$  
        $\equiv (p\land q)\lor r)$
